style: format Internal.Formula

LeanSAT/LRAT/Internal/Formula/Implementation.lean
@@ -13,40 +13,42 @@ namespace Internal
 
 open Assignment DefaultClause Std ReduceResult Std Sat
 
-/-- The structure `DefaultFormula n` takes in a parameter `n` which is intended to be one greater than the total number of variables that
-    can appear in the formula (hence why the parameter `n` is called `numVarsSucc` below). The structure has 4 fields:
-    - The `clauses` field maintains the total set of clauses that appear in the formula. Additionally, when a default formula is created
-      by parsing a CNF file and modified by a series of LRAT additions and deletions, the following informal invariant is maintained:
-      1. `clauses[0]` is always set to `none`.
-      2. The m clauses in the original CNF file are stored in indices 1 through m of the `clauses` field (and they are stored in the order
-         in which they appear in the CNF file).
-      3. Each subsequent LRAT addition is pushed to the very end of the `clauses` array, even if there are elements in the current array set
-         to none.
-      4. When a clause index is deleted via `delete`, that index in `clauses` is set to `none`
+/--
+The structure `DefaultFormula n` takes in a parameter `n` which is intended to be one greater than the total number of variables that
+can appear in the formula (hence why the parameter `n` is called `numVarsSucc` below). The structure has 4 fields:
+- The `clauses` field maintains the total set of clauses that appear in the formula. Additionally, when a default formula is created
+  by parsing a CNF file and modified by a series of LRAT additions and deletions, the following informal invariant is maintained:
+  1. `clauses[0]` is always set to `none`.
+  2. The m clauses in the original CNF file are stored in indices 1 through m of the `clauses` field (and they are stored in the order
+     in which they appear in the CNF file).
+  3. Each subsequent LRAT addition is pushed to the very end of the `clauses` array, even if there are elements in the current array set
+     to none.
+  4. When a clause index is deleted via `delete`, that index in `clauses` is set to `none`
 
-      The purpose of this invariant is to preserve a 1-to-1 correspondence between indices referenced by any external LRAT proof and the internal
-      indices used within `clauses`
+  The purpose of this invariant is to preserve a 1-to-1 correspondence between indices referenced by any external LRAT proof and the internal
+  indices used within `clauses`
 
-    - The `rupUnits` field is empty except during the processing of RUP additions and RAT additions. During a RUP addition or a RAT addition, the
-      `rupUnits` field is used to store negated units from the clause being evaluated for the addition. Regardless of whether the addition is
-      successful, the `rupUnits` field is cleared prior to returning. The reason that `rupUnits` is included as part of the default formula
-      structure (as opposed to simply being an Array that is passed through the helper functions relating to RUP and RAT additions) is to simplify
-      the semantics of default formulas. Since `rupUnits` is part of the default formula structure, it can be taken into account in the `toList`
-      function that defines its satisfiability semantics, making it possible to "add" negated units to a default formula and have it affect its
-      semantics in an easily reversible manner.
+- The `rupUnits` field is empty except during the processing of RUP additions and RAT additions. During a RUP addition or a RAT addition, the
+  `rupUnits` field is used to store negated units from the clause being evaluated for the addition. Regardless of whether the addition is
+  successful, the `rupUnits` field is cleared prior to returning. The reason that `rupUnits` is included as part of the default formula
+  structure (as opposed to simply being an Array that is passed through the helper functions relating to RUP and RAT additions) is to simplify
+  the semantics of default formulas. Since `rupUnits` is part of the default formula structure, it can be taken into account in the `toList`
+  function that defines its satisfiability semantics, making it possible to "add" negated units to a default formula and have it affect its
+  semantics in an easily reversible manner.
 
-    - The `ratUnits` field is empty except during the processing of RAT additions. This field serves an extremely similar role to `rupUnits` in that
-      it is used to temporarily store negated units during unit propogation. The primary difference between the `rupUnits` field and `ratUnits` field
-      is that the `rupUnits` field is only updated twice for each RUP or RAT addition (once to add negated units and then once again to remove said
-      negated units), the `ratUnits` field is updated zero times for each RUP addition and updated m times for each RAT addition where m is the number
-      of negative hints in said RAT addition (i.e. the number of clauses in the formula containing the RAT addition's negated pivot literal).
+- The `ratUnits` field is empty except during the processing of RAT additions. This field serves an extremely similar role to `rupUnits` in that
+  it is used to temporarily store negated units during unit propogation. The primary difference between the `rupUnits` field and `ratUnits` field
+  is that the `rupUnits` field is only updated twice for each RUP or RAT addition (once to add negated units and then once again to remove said
+  negated units), the `ratUnits` field is updated zero times for each RUP addition and updated m times for each RAT addition where m is the number
+  of negative hints in said RAT addition (i.e. the number of clauses in the formula containing the RAT addition's negated pivot literal).
 
-    - The `assignments` field is maintained to quickly look up which values (if any) are entailed for a variable by the formula. At most points in time,
-      (i.e. at all points in time except during a RUP or RAT addition), the `assignments` field must satisfy the `StrongAssignmentsInvariant` defined
-      in Formula.Basic.lean. During RUP and RAT additions, the `assignments` field must satisfy the `AssignmentsInvariant` defined in Formula.Basic.lean.
-      The reason that the `assignments` field is contained as an explicit part of the default formula (as opposed to simply being an Array that is passed
-      through the helper functions concerning unit propogation), is so that the (potentially large) Array does not need to repeatedly be allocated and
-      deallocated. By having the `assignments` Array be a field of the default formula, it is easier to ensure that the Array is used linearly. -/
+- The `assignments` field is maintained to quickly look up which values (if any) are entailed for a variable by the formula. At most points in time,
+  (i.e. at all points in time except during a RUP or RAT addition), the `assignments` field must satisfy the `StrongAssignmentsInvariant` defined
+  in Formula.Basic.lean. During RUP and RAT additions, the `assignments` field must satisfy the `AssignmentsInvariant` defined in Formula.Basic.lean.
+  The reason that the `assignments` field is contained as an explicit part of the default formula (as opposed to simply being an Array that is passed
+  through the helper functions concerning unit propogation), is so that the (potentially large) Array does not need to repeatedly be allocated and
+  deallocated. By having the `assignments` Array be a field of the default formula, it is easier to ensure that the Array is used linearly.
+-/
 @[ext] structure DefaultFormula (numVarsSucc : Nat) where
   clauses : Array (Option (DefaultClause numVarsSucc))
   rupUnits : Array (Literal (PosFin numVarsSucc))
@@ -64,7 +66,8 @@ instance {n : Nat} : Inhabited (DefaultFormula n) where
 def toList {n : Nat} (f : DefaultFormula n) : List (DefaultClause n) :=
   (f.clauses.toList.filterMap id) ++ (f.rupUnits.toList.map unit) ++ (f.ratUnits.toList.map unit)
 
-def ofArray_fold_fn (assignments : Array Assignment) (cOpt : Option (DefaultClause n)) : Array Assignment :=
+def ofArray_fold_fn (assignments : Array Assignment) (cOpt : Option (DefaultClause n)) :
+    Array Assignment :=
   match cOpt with
   | none => assignments
   | some c =>
@@ -73,8 +76,10 @@ def ofArray_fold_fn (assignments : Array Assignment) (cOpt : Option (DefaultClau
     | some (l, true) => assignments.modify l addPosAssignment
     | some (l, false) => assignments.modify l addNegAssignment
 
-/-- Note: This function assumes that the provided `clauses` Array is indexed according to the `clauses` field
-    invariant described in the DefaultFormula doc comment. -/
+/--
+Note: This function assumes that the provided `clauses` Array is indexed according to the `clauses`
+field invariant described in the DefaultFormula doc comment.
+-/
 def ofArray {n : Nat} (clauses : Array (Option (DefaultClause n))) : DefaultFormula n :=
   let assignments := clauses.foldl ofArray_fold_fn (Array.mkArray n unassigned)
   ⟨clauses, #[], #[], assignments⟩
@@ -85,35 +90,45 @@ def insert {n : Nat} (f : DefaultFormula n) (c : DefaultClause n) : DefaultFormu
     | none => ⟨clauses.push c, rupUnits, ratUnits, assignments⟩
     | some (l, true) => ⟨clauses.push c, rupUnits, ratUnits, assignments.modify l addPosAssignment⟩
     | some (l, false) => ⟨clauses.push c, rupUnits, ratUnits, assignments.modify l addNegAssignment⟩
+
 def deleteOne {n : Nat} (f : DefaultFormula n) (id : Nat) : DefaultFormula n :=
   let ⟨clauses, rupUnits, ratUnits, assignments⟩ := f
   match clauses[id]! with
     | none => ⟨clauses, rupUnits, ratUnits, assignments⟩
-    | some ⟨[l], _, _⟩ => ⟨clauses.set! id none, rupUnits, ratUnits, assignments.modify l.1 (removeAssignment l.2)⟩
+    | some ⟨[l], _, _⟩ =>
+      ⟨clauses.set! id none, rupUnits, ratUnits, assignments.modify l.1 (removeAssignment l.2)⟩
     | some _ => ⟨clauses.set! id none, rupUnits, ratUnits, assignments⟩
 
-def delete {n : Nat} (f : DefaultFormula n) (ids : Array Nat) : DefaultFormula n := ids.foldl (fun f id => f.deleteOne id) f
+def delete {n : Nat} (f : DefaultFormula n) (ids : Array Nat) : DefaultFormula n :=
+  ids.foldl (fun f id => f.deleteOne id) f
 
 instance {n : Nat} : Entails (PosFin n) (DefaultFormula n) where
   eval := fun p f => (toList f).all (fun s => p ⊨ s)
 
-def formulaEntails_def {n : Nat} (p : (PosFin n) → Bool) (f : DefaultFormula n) :
+theorem formulaEntails_def {n : Nat} (p : (PosFin n) → Bool) (f : DefaultFormula n) :
   Entails.eval p f = (toList f).all (fun c => p ⊨ c) := Eq.refl (p ⊨ f)
 
 def insertUnit : Array (Literal (PosFin n)) × Array Assignment × Bool →
-  Literal (PosFin n) → Array (Literal (PosFin n)) × Array Assignment × Bool :=
+    Literal (PosFin n) → Array (Literal (PosFin n)) × Array Assignment × Bool :=
   fun (units, assignments, foundContradiction) (l, b) =>
     let curAssignment := assignments[l.1]!
     if hasAssignment b curAssignment then (units, assignments, foundContradiction)
     else (units.push (l, b), assignments.modify l (addAssignment b), foundContradiction || curAssignment != unassigned)
 
-/-- Returns an updated formula f and a bool which indicates whether a contradiction was found in the process of updating f -/
-def insertRupUnits {n : Nat} (f : DefaultFormula n) (ls : CNF.Clause (PosFin n)) : DefaultFormula n × Bool :=
+/--
+Returns an updated formula f and a bool which indicates whether a contradiction was found in the
+process of updating f.
+-/
+def insertRupUnits {n : Nat} (f : DefaultFormula n) (ls : CNF.Clause (PosFin n))
+    : DefaultFormula n × Bool :=
   let ⟨clauses, rupUnits, ratUnits, assignments⟩ := f
   let (rupUnits, assignments, foundContradiction) := ls.foldl insertUnit (rupUnits, assignments, false)
   (⟨clauses, rupUnits, ratUnits, assignments⟩, foundContradiction)
 
-/-- Returns an updated formula f and a bool which indicates whether a contradiction was found in the process of updating f -/
+/--
+Returns an updated formula f and a bool which indicates whether a contradiction was found in the
+process of updating f.
+-/
 def insertRatUnits {n : Nat} (f : DefaultFormula n) (ls : CNF.Clause (PosFin n)) : DefaultFormula n × Bool :=
   let ⟨clauses, rupUnits, ratUnits, assignments⟩ := f
   let (ratUnits, assignments, foundContradiction) := ls.foldl insertUnit (ratUnits, assignments, false)
@@ -132,13 +147,19 @@ def clearRatUnits {n : Nat} (f : DefaultFormula n) : DefaultFormula n :=
   let assignments := ratUnits.foldl clearUnit assignments
   ⟨clauses, rupUnits, #[], assignments⟩
 
-/-- Reverts assignments to the array it was prior to adding derivedLits -/
+/--
+Reverts assignments to the array it was prior to adding derivedLits.
+-/
 def restoreAssignments {n : Nat} (assignments : Array Assignment) (derivedLits : List (PosFin n × Bool)) :
-  Array Assignment := derivedLits.foldl clearUnit assignments
+    Array Assignment :=
+  derivedLits.foldl clearUnit assignments
 
-/-- The fold function used for performRupCheck -/
-def confirmRupHint {n : Nat} (clauses : Array (Option (DefaultClause n))) : Array Assignment × CNF.Clause (PosFin n) × Bool × Bool →
-  Nat → Array Assignment × CNF.Clause (PosFin n) × Bool × Bool :=
+/--
+The fold function used for performRupCheck.
+-/
+def confirmRupHint {n : Nat} (clauses : Array (Option (DefaultClause n))) :
+    Array Assignment × CNF.Clause (PosFin n) × Bool × Bool → Nat →
+    Array Assignment × CNF.Clause (PosFin n) × Bool × Bool :=
   fun (assignments, derivedLits, derivedEmpty, encounteredError) id =>
     if (encounteredError || derivedEmpty) then (assignments, derivedLits, derivedEmpty, encounteredError)
     else
@@ -156,24 +177,30 @@ def confirmRupHint {n : Nat} (clauses : Array (Option (DefaultClause n))) : Arra
       | some none => (assignments, derivedLits, false, true) -- encounteredError
       | none => (assignments, derivedLits, false, true) -- encounteredError
 
-/-- Takes in a formula f and an array of rupHints and attempts to verify that f is unsatisfiable. It returns:
-    - f', which is the same as f but the assignments field has been updated to be consistent with anything learned over the
-      course of the rupCheck
-    - derivedLits, which is the list of literals that were derived over the course of the rupCheck (these are needed to
-      eventually reconstruct the original assignment)
-    - derivedEmpty, which indicates whether the empty clause or a contradiction was derived
-    - encounteredError, which is true if the rupCheck failed and false otherwise
+/--
+Takes in a formula f and an array of rupHints and attempts to verify that f is unsatisfiable. It returns:
+- f', which is the same as f but the assignments field has been updated to be consistent with anything learned over the
+  course of the rupCheck
+- derivedLits, which is the list of literals that were derived over the course of the rupCheck (these are needed to
+  eventually reconstruct the original assignment)
+- derivedEmpty, which indicates whether the empty clause or a contradiction was derived
+- encounteredError, which is true if the rupCheck failed and false otherwise
 
-    Note: This function assumes that any rupUnits and ratUnits corresponding to this rup check have already been added to f. -/
+Note: This function assumes that any rupUnits and ratUnits corresponding to this rup check have already been added to f.
+-/
 def performRupCheck {n : Nat} (f : DefaultFormula n) (rupHints : Array Nat) :
-  DefaultFormula n × CNF.Clause (PosFin n) × Bool × Bool :=
+    DefaultFormula n × CNF.Clause (PosFin n) × Bool × Bool :=
   let ⟨clauses, rupUnits, ratUnits, assignments⟩ := f
   let (assignments, derivedLits, derivedEmpty, encounteredError) := rupHints.foldl (confirmRupHint clauses) (assignments, [], false, false)
   (⟨clauses, rupUnits, ratUnits, assignments⟩, derivedLits, derivedEmpty, encounteredError)
 
-/-- Attempts to verify that c can be added to f via unit propagation. If it can, it returns ((f.insert c), true). If it can't,
-    it returns false as the second part of the tuple (and no guarantees are made about what formula is returned) -/
-def performRupAdd {n : Nat} (f : DefaultFormula n) (c : DefaultClause n) (rupHints : Array Nat) : DefaultFormula n × Bool :=
+/--
+Attempts to verify that c can be added to f via unit propagation. If it can, it returns
+`((f.insert c), true)`. If it can't, it returns false as the second part of the tuple
+(and no guarantees are made about what formula is returned).
+-/
+def performRupAdd {n : Nat} (f : DefaultFormula n) (c : DefaultClause n) (rupHints : Array Nat) :
+    DefaultFormula n × Bool :=
   let negC := negate c
   let (f, foundContradiction) := insertRupUnits f negC
   if foundContradiction then
@@ -192,7 +219,9 @@ def performRupAdd {n : Nat} (f : DefaultFormula n) (c : DefaultClause n) (rupHin
       (f.insert c, true)
 
 /-- Returns an array of indices corresponding to clauses that contain the negation of l -/
-def getRatClauseIndices {n : Nat} (clauses : Array (Option (DefaultClause n))) (l : Literal (PosFin n)) : Array Nat :=
+def getRatClauseIndices {n : Nat} (clauses : Array (Option (DefaultClause n)))
+    (l : Literal (PosFin n)) :
+    Array Nat :=
   let negL := Literal.negate l
   let filter_fn := fun i =>
     match clauses[i]! with
@@ -200,23 +229,33 @@ def getRatClauseIndices {n : Nat} (clauses : Array (Option (DefaultClause n))) (
     | some c => c.contains negL
   (Array.range clauses.size).filter filter_fn
 
-/-- Checks that for each clause c ∈ f such that (Literal.negate pivot) ∈ c, c's index is in ratHints.map (fun x => x.1). This
-    function assumes that ratHints are ordered by the value of their first argument, which is consistent with LRAT's specification -/
-def ratHintsExhaustive {n : Nat} (f : DefaultFormula n) (pivot : Literal (PosFin n)) (ratHints : Array (Nat × Array Nat)) : Bool :=
+/--
+Checks that for each clause `c ∈ f` such that `(Literal.negate pivot) ∈ c`, `c`'s index is in
+`ratHints.map (fun x => x.1)`. This function assumes that ratHints are ordered by the value of their
+first argument, which is consistent with LRAT's specification
+-/
+def ratHintsExhaustive {n : Nat} (f : DefaultFormula n) (pivot : Literal (PosFin n))
+    (ratHints : Array (Nat × Array Nat)) :
+    Bool :=
   let ratClauseIndices := getRatClauseIndices f.clauses pivot
   let ratHintIndices := ratHints.map (fun x => x.1) -- This doesn't use ratHints linearly ratHints shouldn't be large
   ratClauseIndices = ratHintIndices
 
-/-- Takes in a formula f and a single ratHint and attempts to verify that f is inconsistent with the negation of the ratHint's
-    clause. It returns:
-    - f which is the same as the original f (including the ratUnits and assignment fields)
-      - Although the ratUnits and assignments fields are updated during the procedure, they are restored prior to returning
-    - success, which indicates whether empty was successfully derived without any errors
+/--
+Takes in a formula `f` and a single `ratHint` and attempts to verify that `f` is inconsistent with the
+negation of the `ratHint`'s clause. It returns:
+- `f` which is the same as the original `f` (including the ratUnits and assignment fields)
+  - Although the `ratUnits` and `assignments` fields are updated during the procedure,
+    they are restored prior to returning..
+- `success`, which indicates whether empty was successfully derived without any errors
 
-    Note: This function assumes that the ratUnits corresponding to this rat check have NOT already been added to f. In terms of
-    input expectations and output guarantees, this function is more analogous to performRupAdd than performRupCheck -/
-def performRatCheck {n : Nat} (f : DefaultFormula n) (negPivot : Literal (PosFin n)) (ratHint : Nat × Array Nat) :
-  DefaultFormula n × Bool :=
+Note: This function assumes that the `ratUnits` corresponding to this rat check have NOT already
+been added to `f`. In terms of input expectations and output guarantees, this function is more
+analogous to `performRupAdd` than `performRupCheck`.
+-/
+def performRatCheck {n : Nat} (f : DefaultFormula n) (negPivot : Literal (PosFin n))
+    (ratHint : Nat × Array Nat) :
+    DefaultFormula n × Bool :=
   match f, ratHint with
   | ⟨clauses, rupUnits, ratUnits, assignments⟩, (id, rupHints) =>
     match clauses[id]! with
@@ -238,10 +277,14 @@ def performRatCheck {n : Nat} (f : DefaultFormula n) (negPivot : Literal (PosFin
           else (f, true)
     | none => (⟨clauses, rupUnits, ratUnits, assignments⟩, false)
 
-/-- Attempts to verify that c can be added to f via unit propagation. If it can, it returns ((f.insert c), true). If it can't,
-    it returns false as the second part of the tuple (and no guarantees are made about what formula is returned) -/
-def performRatAdd {n : Nat} (f : DefaultFormula n) (c : DefaultClause n) (pivot : Literal (PosFin n)) (rupHints : Array Nat)
-  (ratHints : Array (Nat × Array Nat)) : DefaultFormula n × Bool :=
+/--
+Attempts to verify that `c` can be added to `f` via unit propagation. If it can, it returns
+`((f.insert c), true)`. If it can't, it returns false as the second part of the tuple
+(and no guarantees are made about what formula is returned).
+-/
+def performRatAdd {n : Nat} (f : DefaultFormula n) (c : DefaultClause n)
+    (pivot : Literal (PosFin n)) (rupHints : Array Nat) (ratHints : Array (Nat × Array Nat)) :
+    DefaultFormula n × Bool :=
   if ratHintsExhaustive f pivot ratHints then
     let negC := negate c
     let (f, contradictionFound) := insertRupUnits f negC
